monads: Monad as Functor.

monads/Monad.v
@@ -1,3 +1,6 @@
+Require Import Coq.Logic.FunctionalExtensionality.
+Require Import Coq.Program.Basics.
+
 Set Implicit Arguments.
 
 Module Type Monad.
@@ -15,13 +18,13 @@ Module Type Monad.
     Law 1:  return x >>= f ~ f x
     Law 2:  m >>= return ~ m
     Law 3:  (m >>= f) >>= g ~ m >>= (fun x -> f x >>= g) *)
-  Axiom monad_law1 : forall (A B : Type) (x : A) (f : A -> m B),
+  Axiom law1 : forall (A B : Type) (x : A) (f : A -> m B),
     ret x >>= f = f x.
 
-  Axiom monad_law2 : forall (A : Type) (x : m A),
+  Axiom law2 : forall (A : Type) (x : m A),
     x >>= @ret A = x.
 
-  Axiom monad_law3 :
+  Axiom law3 :
     forall (A B C : Type) (n : m A) (f : A -> m B) (g : B -> m C),
       (n >>= f) >>= g = n >>= (fun x => f x >>= g).
 End Monad.
@@ -30,9 +33,42 @@ End Monad.
 Module MonadExt (M : Monad).
   Import M.
 
+  Definition id (A : Type) := fun (x : A) => x.
+
   Definition fmap (A B : Type) (f : A -> B) (n : m A) : m B :=
-    n >>= (fun x => ret (f x)).
+    n >>= compose (@ret B) f.
 
   Definition join (A : Type) (n : m (m A)) : m A :=
-    n >>= (fun x => x).
+    n >>= @id (m A).
+
+  Theorem fmap_compose_join_eq_bind :
+    forall (A B : Type) (n : m A) (f : A -> m B),
+      n >>= f = join (fmap f n).
+  Proof.
+    unfold join, fmap; intros.
+    rewrite law3.
+    f_equal; apply functional_extensionality; intros.
+    unfold compose; rewrite law1.
+    auto.
+  Qed.
+
+  (** Properties for Monad as a Functor. *)
+  Theorem fmap_id :
+    forall (A : Type), fmap (@id A) = @id (m A).
+  Proof.
+    unfold fmap; intros.
+    apply functional_extensionality; intros; unfold id.
+    rewrite law2. auto.
+  Qed.
+
+  Theorem fmap_associativity :
+    forall (A B C : Type) (f : A -> B) (g : B -> C),
+      fmap (compose g f) = compose (fmap g) (fmap f).
+  Proof.
+    unfold fmap, compose; intros.
+    apply functional_extensionality; intros.
+    rewrite law3; f_equal.
+    apply functional_extensionality; intros.
+    rewrite law1. auto.
+  Qed.
 End MonadExt.
